refact

fizzBuzz.fst
@@ -12,49 +12,50 @@ module U = FStar.UInt
 module U32 = FStar.UInt32
 module ST = FStar.HyperStack.ST
 
-val create_fizzBuzz_array: src:B.buffer string -> n:U32.t -> Stack C.exit_code
-(requires fun h0 -> B.live h0 src /\ B.length src = U32.v n )
+val create_fizzBuzz_array: fizzBuzz_array:B.buffer string -> n:U32.t -> Stack C.exit_code
+(requires fun h0 -> B.live h0 fizzBuzz_array /\ B.length fizzBuzz_array = U32.v n )
 (ensures fun _ _ _ -> true)
-let create_fizzBuzz_array src n =
-  let inv h (i: nat) = B.live h src in
+let create_fizzBuzz_array fizzBuzz_array n =
+  let inv h (i: nat) = B.live h fizzBuzz_array in
   let body (i: U32.t{ 0 <= U32.v i /\ U32.v i < U32.v n }): Stack unit
     (requires (fun h -> inv h (U32.v i)))
     (ensures (fun _ _ _ -> true))
   =
-    let v : string = src.(i) in
+    let v : string = fizzBuzz_array.(i) in
     let count: U32.t = U32.(i +^ 1ul) in
-    let fillStr (x:string) = src.(i) <- x in
+    let fillStr (x:string) = fizzBuzz_array.(i) <- x in
     let u32Mod (a: U32.t) (b: U32.t{b <> 0ul}) = U32.uint_to_t (U.mod (U32.v a) (U32.v b)) in
       if u32Mod count 15ul = 0ul then (fillStr "FizzBuzz")  
       else if u32Mod count 3ul = 0ul then (fillStr "Fizz")  
       else if u32Mod count 5ul = 0ul then (fillStr "Buzz") 
   in
   C.Loops.for 0ul n inv body;
-  (* return *) C.EXIT_SUCCESS
+  C.EXIT_SUCCESS
 
-val decorate_fizzBuzz_array: src:B.buffer string -> n:U32.t -> Stack C.exit_code
-  (requires fun h0 -> B.live h0 src /\ B.length src = U32.v n )
+val decorate_fizzBuzz_array: fizzBuzz_array:B.buffer string -> n:U32.t -> Stack C.exit_code
+  (requires fun h0 -> B.live h0 fizzBuzz_array /\ B.length fizzBuzz_array = U32.v n )
   (ensures fun _ _ _ -> true)
-let decorate_fizzBuzz_array src n =
-  let inv h (i: nat) = B.live h src in
+let decorate_fizzBuzz_array fizzBuzz_array n =
+  let inv h (i: nat) = B.live h fizzBuzz_array in
   let body (i: U32.t{ 0 <= U32.v i /\ U32.v i < U32.v n }): Stack unit
     (requires (fun h -> inv h (U32.v i)))
     (ensures (fun _ _ _ -> true))
   =
-    let v : string = src.(i) in
+    let v : string = fizzBuzz_array.(i) in
     let count: U32.t = U32.(i +^ 1ul) in
-    printf "%ul: %s\n" count v done
+    if v = "" then printf "%ul\n" count done
+    else printf "%s\n" v  done
   in
   C.Loops.for 0ul n inv body;
-  (* return *) C.EXIT_SUCCESS
+  C.EXIT_SUCCESS
 
 let main ()
 =
   push_frame ();
-  let n = 10ul in
+  let n = 30ul in
   let fillData = "" in
-  let src = B.alloca fillData n in
-  let _ = create_fizzBuzz_array src n in
-  let _ = decorate_fizzBuzz_array src n in
+  let fizzBuzz_array = B.alloca fillData n in
+  let _ = create_fizzBuzz_array fizzBuzz_array n in
+  let _ = decorate_fizzBuzz_array fizzBuzz_array n in
   pop_frame ();
   C.EXIT_SUCCESS
